Move spec of MLDSA arithmetic to Spec.MLDSA.Math

libcrux-ml-dsa/src/simd/portable/arithmetic.rs
@@ -254,14 +254,9 @@ pub(crate) fn montgomery_multiply(lhs: &mut Coefficients, rhs: &Coefficients) {
 #[inline(always)]
 #[hax_lib::fstar::options("--ext context_pruning --z3refresh --split_queries always")]
 #[hax_lib::requires(fstar!(r#"Spec.Utils.is_i32b (v $FIELD_MODULUS - 1) $t"#))]
-#[hax_lib::ensures(|(t0,t1)| fstar!(r#"
-    v $t0 == Spec.Utils.mod_q (v $t % v $FIELD_MODULUS) (pow2 (v $BITS_IN_LOWER_PART_OF_T)) /\
-    v $t1 == ((v $t % v $FIELD_MODULUS) - v $t0) / pow2 (v $BITS_IN_LOWER_PART_OF_T) /\
-    v $t0 > -(pow2 (v $BITS_IN_LOWER_PART_OF_T - 1)) /\ v $t0 <= pow2 (v $BITS_IN_LOWER_PART_OF_T - 1)"#))]
+#[hax_lib::ensures(|(t0,t1)| fstar!(r#"let (t0_s, t1_s) = Spec.MLDSA.Math.power2round (v $t) in
+    v $t0 == t0_s /\ v $t1 == t1_s /\ Spec.Utils.is_intb_bt (pow2 (v $BITS_IN_LOWER_PART_OF_T - 1)) (v $t0)"#))]
 fn power2round_element(t: i32) -> (i32, i32) {
-    // Hax issue: https://github.com/hacspec/hax/issues/1082
-    debug_assert!(t > -FIELD_MODULUS && t < FIELD_MODULUS);
-
     hax_lib::fstar!(
         "logand_lemma $FIELD_MODULUS (t >>! mk_i32 31)");
     let _t = t;
@@ -278,23 +273,23 @@ fn power2round_element(t: i32) -> (i32, i32) {
     let t1 = (t - 1 + (1 << (BITS_IN_LOWER_PART_OF_T - 1))) >> BITS_IN_LOWER_PART_OF_T;
     hax_lib::fstar!(
         "assert (v $t1 == (v $t - 1 + pow2 12) / pow2 13);
-        assert ((v $t - (Spec.Utils.mod_q (v $t) (pow2 13))) / pow2 13 ==
-            (v $t / pow2 13 - (Spec.Utils.mod_q (v $t) (pow2 13)) / pow2 13));
+        assert ((v $t - (Spec.Utils.mod_p (v $t) (pow2 13))) / pow2 13 ==
+            (v $t / pow2 13 - (Spec.Utils.mod_p (v $t) (pow2 13)) / pow2 13));
         if v $t % pow2 13 > pow2 12 then
-            (assert (Spec.Utils.mod_q (v $t) (pow2 13) == v $t % pow2 13 - pow2 13);
-            assert ((Spec.Utils.mod_q (v $t) (pow2 13)) / pow2 13 == (v $t % pow2 13 - pow2 13) / pow2 13);
+            (assert (Spec.Utils.mod_p (v $t) (pow2 13) == v $t % pow2 13 - pow2 13);
+            assert ((Spec.Utils.mod_p (v $t) (pow2 13)) / pow2 13 == (v $t % pow2 13 - pow2 13) / pow2 13);
             assert ((v $t % pow2 13 - pow2 13) / pow2 13 == (v $t % pow2 13) / pow2 13 - pow2 13 / pow2 13);
             assert ((v $t % pow2 13) / pow2 13 - pow2 13 / pow2 13 == -1);
-            assert ((v $t - (Spec.Utils.mod_q (v $t) (pow2 13))) / pow2 13 == v $t / pow2 13 + 1))
+            assert ((v $t - (Spec.Utils.mod_p (v $t) (pow2 13))) / pow2 13 == v $t / pow2 13 + 1))
         else
-            (assert ((v $t - (Spec.Utils.mod_q (v $t) (pow2 13))) / pow2 13 == v $t / pow2 13);
+            (assert ((v $t - (Spec.Utils.mod_p (v $t) (pow2 13))) / pow2 13 == v $t / pow2 13);
             assert ((v $t - 1 + pow2 12) / pow2 13 == v $t / pow2 13));
-        assert (v $t1 == (v $t - (Spec.Utils.mod_q (v $t) (pow2 13))) / pow2 13)");
+        assert (v $t1 == (v $t - (Spec.Utils.mod_p (v $t) (pow2 13))) / pow2 13)");
     let t0 = t - (t1 << BITS_IN_LOWER_PART_OF_T);
     hax_lib::fstar!(
-        "assert (v $t0 == v $t - ((v $t - (Spec.Utils.mod_q (v $t) (pow2 13))) / pow2 13) * pow2 13);
-        assert (v $t0 == v $t - (v $t - (Spec.Utils.mod_q (v $t) (pow2 13))));
-        assert (v $t0 == Spec.Utils.mod_q (v $t) (pow2 13))");
+        "assert (v $t0 == v $t - ((v $t - (Spec.Utils.mod_p (v $t) (pow2 13))) / pow2 13) * pow2 13);
+        assert (v $t0 == v $t - (v $t - (Spec.Utils.mod_p (v $t) (pow2 13))));
+        assert (v $t0 == Spec.Utils.mod_p (v $t) (pow2 13))");
 
     (t0, t1)
 }
@@ -303,21 +298,19 @@ fn power2round_element(t: i32) -> (i32, i32) {
 #[hax_lib::requires(fstar!(r#"Spec.Utils.is_i32b_array (v $FIELD_MODULUS - 1) ${t0}.f_values"#))]
 #[hax_lib::ensures(|_| fstar!(r#"
     forall i. i < 8 ==>
-        (let t0_1 = v (Seq.index ${t0}.f_values i) % v $FIELD_MODULUS in
-        let t0_2 = v (Seq.index ${t0}_future.f_values i) in
-        t0_2 == Spec.Utils.mod_q t0_1 (pow2 (v $BITS_IN_LOWER_PART_OF_T)) /\
-        v (Seq.index ${t1}_future.f_values i) == (t0_1 - t0_2) / pow2 (v $BITS_IN_LOWER_PART_OF_T) /\
-        t0_2 > -(pow2 (v $BITS_IN_LOWER_PART_OF_T - 1)) /\ t0_2 <= pow2 (v $BITS_IN_LOWER_PART_OF_T - 1))"#))]
+        (let t0_v = v (Seq.index ${t0}_future.f_values i) in
+        let (t0_s, t1_s) = Spec.MLDSA.Math.power2round (v (Seq.index ${t0}.f_values i)) in
+        t0_v == t0_s /\ v (Seq.index ${t1}_future.f_values i) == t1_s /\
+        Spec.Utils.is_intb_bt (pow2 (v $BITS_IN_LOWER_PART_OF_T - 1)) t0_v)"#))]
 pub(super) fn power2round(t0: &mut Coefficients, t1: &mut Coefficients) {
     let _t0: Coefficients = t0.clone();
     for i in 0..t0.values.len() {
         hax_lib::loop_invariant!(|i: usize| {
             fstar!(r#"
-                (forall j. j < v i ==> (let t0_1 = v (Seq.index ${_t0}.f_values j) % v $FIELD_MODULUS in
-                    let t0_2 = v (Seq.index ${t0}.f_values j) in
-                    t0_2 == Spec.Utils.mod_q t0_1 (pow2 (v $BITS_IN_LOWER_PART_OF_T)) /\
-                    v (Seq.index ${t1}.f_values j) == (t0_1 - t0_2) / pow2 (v $BITS_IN_LOWER_PART_OF_T) /\
-                    t0_2 > -(pow2 (v $BITS_IN_LOWER_PART_OF_T - 1)) /\ t0_2 <= pow2 (v $BITS_IN_LOWER_PART_OF_T - 1))) /\
+                (forall j. j < v i ==> (let t0_v = v (Seq.index ${t0}.f_values j) in
+                    let (t0_s, t1_s) = Spec.MLDSA.Math.power2round (v (Seq.index ${_t0}.f_values j)) in
+                    t0_v == t0_s /\ v (Seq.index ${t1}.f_values j) == t1_s /\
+                    Spec.Utils.is_intb_bt (pow2 (v $BITS_IN_LOWER_PART_OF_T - 1)) t0_v)) /\
                 (forall j. j >= v i ==> (Seq.index ${t0}.f_values j == Seq.index ${_t0}.f_values j /\
                     Spec.Utils.is_i32b (v $FIELD_MODULUS - 1) (Seq.index ${t0}.f_values j)))"#
             )
@@ -346,7 +339,6 @@ pub(super) fn infinity_norm_exceeds(simd_unit: &Coefficients, bound: i32) -> boo
             )
         });
         let coefficient = simd_unit.values[i];
-        debug_assert!(coefficient > -FIELD_MODULUS && coefficient < FIELD_MODULUS);
         // This norm is calculated using the absolute value of the
         // signed representative in the range:
         //
@@ -419,12 +411,7 @@ pub(super) fn shift_left_then_reduce<const SHIFT_BY: i32>(simd_unit: &mut Coeffi
 
 #[inline(always)]
 #[hax_lib::requires(fstar!(r#"v $gamma2 == v $GAMMA2_V261_888 \/ v $gamma2 == v $GAMMA2_V95_232"#))]
-#[hax_lib::ensures(|result| fstar!(r#"if
-    v $low > v $gamma2 || v $low < -(v $gamma2) || (v $low = -(v $gamma2) && v $high <> 0)
-    then
-        v $result = 1
-    else
-        v $result = 0"#))]
+#[hax_lib::ensures(|result| fstar!(r#"v $result = Spec.MLDSA.Math.compute_one_hint (v $low) (v $high) (v $gamma2)"#))]
 fn compute_one_hint(low: i32, high: i32, gamma2: i32) -> i32 {
     if (low > gamma2) || (low < -gamma2) || (low == -gamma2 && high != 0) {
         1
@@ -433,46 +420,13 @@ fn compute_one_hint(low: i32, high: i32, gamma2: i32) -> i32 {
     }
 }
 
-#[cfg_attr(hax, hax_lib::fstar::before(interface,
-r#"let hint_counter (hint:t_Array i32 (mk_usize 8)) (i:nat{i < 8}) (s:nat) : Tot (nat) =
-  s + v (cast hint.[sz i] <: usize)"#
-))]
-#[cfg_attr(hax, hax_lib::fstar::before(
-r#"val hint_counter_loop:
-  hint_1:t_Array i32 (mk_usize 8)
-  -> hint_2:t_Array i32 (mk_usize 8)
-  -> n:nat{n < 8} ->
-  Lemma
-   (requires
-      forall (i:nat). i < n ==> hint_1.[mk_usize i] == hint_2.[mk_usize i])
-    (ensures
-      Lib.LoopCombinators.repeati n (hint_counter hint_1) 0 ==
-        Lib.LoopCombinators.repeati n (hint_counter hint_2) 0)
-
-let rec hint_counter_loop hint_1 hint_2 n =
-  if n = 0 then begin
-    Lib.LoopCombinators.eq_repeati0 n (hint_counter hint_1) 0;
-    Lib.LoopCombinators.eq_repeati0 n (hint_counter hint_2) 0;
-    () end
-  else begin
-    hint_counter_loop hint_1 hint_2 (n - 1);
-    Lib.LoopCombinators.unfold_repeati n (hint_counter hint_1) 0 (n - 1);
-    Lib.LoopCombinators.unfold_repeati n (hint_counter hint_2) 0 (n - 1);
-    () end"#
-))]
 #[inline(always)]
 #[hax_lib::requires(fstar!(r#"v $gamma2 == v $GAMMA2_V261_888 \/ v $gamma2 == v $GAMMA2_V95_232"#))]
 #[hax_lib::ensures(|result| fstar!(r#"
-    (forall i. i < 8 ==> (let r = v (Seq.index ${hint}_future.f_values i) in
-        let l = v (Seq.index ${low}.f_values i) in
-        let h = v (Seq.index ${high}.f_values i) in
-        if l > v $gamma2 || l < -(v $gamma2) || 
-        (l = -(v $gamma2) && h <> 0)
-        then
-            r = 1
-        else
-            r = 0)) /\
-    v $result == Lib.LoopCombinators.repeati 8 (hint_counter ${hint}_future.f_values) 0"#
+    (forall i. i < 8 ==> (v (Seq.index ${hint}_future.f_values i) =
+        Spec.MLDSA.Math.compute_one_hint (v (Seq.index ${low}.f_values i))
+            (v (Seq.index ${high}.f_values i)) (v $gamma2))) /\
+    v $result == Spec.MLDSA.Math.compute_hint ${hint}_future.f_values"#
 ))]
 pub(super) fn compute_hint(
     low: &Coefficients,
@@ -483,30 +437,24 @@ pub(super) fn compute_hint(
     let mut one_hints_count = 0;
 
     hax_lib::fstar!(
-        r#"Lib.LoopCombinators.eq_repeati0 0 (hint_counter ${hint}.f_values) 0"#
+        r#"Lib.LoopCombinators.eq_repeati0 0 (Spec.MLDSA.Math.hint_counter ${hint}.f_values) 0"#
     );
     for i in 0..hint.values.len() {
         hax_lib::loop_invariant!(|i: usize| {
             fstar!(r#"
                 v $i >= 0 /\ v $i <= 8 /\
-                (forall j. j < v i ==> (let r = v (Seq.index ${hint}.f_values j) in
-                    let l = v (Seq.index ${low}.f_values j) in
-                    let h = v (Seq.index ${high}.f_values j) in
-                    if l > v $gamma2 || l < -(v $gamma2) || 
-                    (l = -(v $gamma2) && h <> 0)
-                    then
-                        r = 1
-                    else
-                        r = 0)) /\
+                (forall j. j < v i ==> (v (Seq.index ${hint}.f_values j) =
+                    Spec.MLDSA.Math.compute_one_hint (v (Seq.index ${low}.f_values j))
+                        (v (Seq.index ${high}.f_values j)) (v $gamma2))) /\
                 v $one_hints_count <= v $i /\
-                v $one_hints_count == Lib.LoopCombinators.repeati (v $i) (hint_counter ${hint}.f_values) 0"#
+                v $one_hints_count == Lib.LoopCombinators.repeati (v $i) (Spec.MLDSA.Math.hint_counter ${hint}.f_values) 0"#
             )
         });
         let _hint_values = hint.values;
         hint.values[i] = compute_one_hint(low.values[i], high.values[i], gamma2);
         hax_lib::fstar!(
-            r#"hint_counter_loop ${hint}.f_values $_hint_values (v i);
-            Lib.LoopCombinators.unfold_repeati (v $i + 1) (hint_counter ${hint}.f_values) 0 (v $i)"#
+            r#"Spec.MLDSA.Math.hint_counter_loop ${hint}.f_values $_hint_values (v i);
+            Lib.LoopCombinators.unfold_repeati (v $i + 1) (Spec.MLDSA.Math.hint_counter ${hint}.f_values) 0 (v $i)"#
         );
         one_hints_count += hint.values[i] as usize;
     }
@@ -529,22 +477,18 @@ pub(super) fn compute_hint(
 //
 // Note that 0 ≤ r₁ < (q-1)/α.
 #[inline(always)]
-#[hax_lib::fstar::options("--fuel 3 --z3rlimit 500 --ext context_pruning --z3refresh --split_queries always")]
+#[hax_lib::fstar::options("--fuel 3 --z3rlimit 1500 --ext context_pruning --z3refresh --split_queries always")]
 #[hax_lib::requires(fstar!(r#"(v $gamma2 == v $GAMMA2_V261_888 \/ v $gamma2 == v $GAMMA2_V95_232) /\
     Spec.Utils.is_i32b (v $FIELD_MODULUS - 1) $r"#))]
 #[hax_lib::ensures(|(r0,r1)| fstar!(r#"
-    let r_q = v $r % v $FIELD_MODULUS in
-    let r_g = Spec.Utils.mod_q r_q (v $gamma2 * 2) in
-    (if r_q - r_g = v $FIELD_MODULUS - 1 then
-        (v $r0 == r_g - 1 /\ v $r1 == 0 /\
-        (v $r0 >= -(v $gamma2) /\ v $r0 < 0))
+    let (r0_s, r1_s, cond) = Spec.MLDSA.Math.decompose (v $gamma2) (v $r) in
+    v $r0 = r0_s /\ v $r1 = r1_s /\
+    (if cond then
+        (v $r0 >= -(v $gamma2) /\ v $r0 < 0)
     else
-        (v $r0 == r_g /\ v $r1 == (r_q - r_g) / (v $gamma2 * 2) /\
-        (v $r0 > -(v $gamma2) /\ v $r0 <= v $gamma2))) /\
+        (v $r0 > -(v $gamma2) /\ v $r0 <= v $gamma2)) /\
     (v $r1 >= 0 /\ v $r1 < (v $FIELD_MODULUS - 1) / (v $gamma2 * 2))"#))]
 fn decompose_element(gamma2: Gamma2, r: i32) -> (i32, i32) {
-    debug_assert!(r > -FIELD_MODULUS && r < FIELD_MODULUS);
-
     let _r = r;
     hax_lib::fstar!(
         r#"logand_lemma $FIELD_MODULUS ($r >>! mk_i32 31)"#
@@ -571,7 +515,7 @@ fn decompose_element(gamma2: Gamma2, r: i32) -> (i32, i32) {
                     r#"assert (v $result == ((v $ceil_of_r_by_128 * 11275) + pow2 23) / pow2 24);
                     assert (v $result == ((((v $r + 127) / 128) * 11275) + pow2 23) / pow2 24);
                     assert (v $result == (v $r - 1 + 95232) / 190464);
-                    assert (v $result == (v $r - (Spec.Utils.mod_q (v $r) 190464)) / 190464);
+                    assert (v $result == (v $r - (Spec.Utils.mod_p (v $r) 190464)) / 190464);
                     assert (v $result >= 0 /\ v $result <= 44)"#
                 );
 
@@ -597,7 +541,7 @@ fn decompose_element(gamma2: Gamma2, r: i32) -> (i32, i32) {
                     r#"assert (v $result == ((v $ceil_of_r_by_128 * 1025) + pow2 21) / pow2 22);
                     assert (v $result == ((((v $r + 127) / 128) * 1025) + pow2 21) / pow2 22);
                     assert (v $result == (v $r - 1 + 261888) / 523776);
-                    assert (v $result == (v $r - (Spec.Utils.mod_q (v $r) 523776)) / 523776);
+                    assert (v $result == (v $r - (Spec.Utils.mod_p (v $r) 523776)) / 523776);
                     assert (v $result >= 0 /\ v $result <= 16)"#
                 );
 
@@ -634,13 +578,13 @@ fn decompose_element(gamma2: Gamma2, r: i32) -> (i32, i32) {
     hax_lib::fstar!(
         r#"assert (v $_r0 > 4190208 ==> v $r0 == v $_r0 - 8380417);
         assert (v $_r0 <= 4190208 ==> v $r0 == v $_r0);
-        if v $r - (Spec.Utils.mod_q (v $r) (v $alpha)) = 8380416 then
+        if v $r - (Spec.Utils.mod_p (v $r) (v $alpha)) = 8380416 then
             (assert (v $r1 == 0);
-            assert (v $r0 == (Spec.Utils.mod_q (v $r) (v $alpha)) - 1);
+            assert (v $r0 == (Spec.Utils.mod_p (v $r) (v $alpha)) - 1);
             assert (v $r0 >= -(v $gamma2) /\ v $r0 < 0))
         else
-            (assert (v $r1 == (v $r - (Spec.Utils.mod_q (v $r) (v $alpha))) / v $alpha);
-            assert (v $r0 == Spec.Utils.mod_q (v $r) (v $alpha));
+            (assert (v $r1 == (v $r - (Spec.Utils.mod_p (v $r) (v $alpha))) / v $alpha);
+            assert (v $r0 == Spec.Utils.mod_p (v $r) (v $alpha));
             assert (v $r0 > -(v $gamma2) /\ v $r0 <= v $gamma2));
         assert (v $r1 >= 0 /\ v $r1 < 8380416 / (v $alpha))"#
     );
@@ -652,14 +596,7 @@ fn decompose_element(gamma2: Gamma2, r: i32) -> (i32, i32) {
 #[hax_lib::requires(fstar!(r#"(v $gamma2 == v $GAMMA2_V261_888 \/ v $gamma2 == v $GAMMA2_V95_232) /\
     Spec.Utils.is_i32b (v $FIELD_MODULUS - 1) $r /\
     (v $hint == 0 \/ v $hint == 1)"#))]
-#[hax_lib::ensures(|result| fstar!(r#"let r0, r1 = decompose_element $gamma2 $r in
-    if v $hint = 0 then
-        $result = r1
-    else
-        (if v r0 > 0 then
-            v $result = (v r1 + 1) % (4190208 / v $gamma2)
-        else
-            v $result = (v r1 - 1) % (4190208 / v $gamma2))"#))]
+#[hax_lib::ensures(|result| fstar!(r#"v $result == Spec.MLDSA.Math.use_one_hint (v $gamma2) (v $r) (v $hint)"#))]
 pub(crate) fn use_one_hint(gamma2: Gamma2, r: i32, hint: i32) -> i32 {
     let (r0, r1) = decompose_element(gamma2, r);
 
@@ -705,14 +642,12 @@ pub(crate) fn use_one_hint(gamma2: Gamma2, r: i32, hint: i32) -> i32 {
     (let r = v (Seq.index ${simd_unit}.f_values i) in
     let r0 = v (Seq.index ${low}_future.f_values i) in
     let r1 = v (Seq.index ${high}_future.f_values i) in
-    let r_q = r % v $FIELD_MODULUS in
-    let r_g = Spec.Utils.mod_q r_q (v $gamma2 * 2) in
-    (if r_q - r_g = v $FIELD_MODULUS - 1 then
-        (r0 == r_g - 1 /\ r1 == 0 /\
-        (r0 >= -(v $gamma2) /\ r0 < 0))
+    let (r0_s, r1_s, cond) = Spec.MLDSA.Math.decompose (v $gamma2) r in
+    r0 = r0_s /\ r1 = r1_s /\
+    (if cond then
+        (r0 >= -(v $gamma2) /\ r0 < 0)
     else
-        (r0 == r_g /\ r1 == (r_q - r_g) / (v $gamma2 * 2) /\
-        (r0 > -(v $gamma2) /\ r0 <= v $gamma2))) /\
+        (r0 > -(v $gamma2) /\ r0 <= v $gamma2)) /\
     (r1 >= 0 /\ r1 < (v $FIELD_MODULUS - 1) / (v $gamma2 * 2)))"#))]
 pub fn decompose(
     gamma2: Gamma2,
@@ -720,21 +655,18 @@ pub fn decompose(
     low: &mut Coefficients,
     high: &mut Coefficients,
 ) {
-    let _simd_unit0 = simd_unit;
     for i in 0..low.values.len() {
         hax_lib::loop_invariant!(|i: usize| {
             fstar!(r#"
                 forall j. j < v i ==> (let r = v (Seq.index ${simd_unit}.f_values j) in
                     let r0 = v (Seq.index ${low}.f_values j) in
                     let r1 = v (Seq.index ${high}.f_values j) in
-                    let r_q = r % v $FIELD_MODULUS in
-                    let r_g = Spec.Utils.mod_q r_q (v $gamma2 * 2) in
-                    (if r_q - r_g = v $FIELD_MODULUS - 1 then
-                        (r0 == r_g - 1 /\ r1 == 0 /\
-                        (r0 >= -(v $gamma2) /\ r0 < 0))
+                    let (r0_s, r1_s, cond) = Spec.MLDSA.Math.decompose (v $gamma2) r in
+                    r0 = r0_s /\ r1 = r1_s /\
+                    (if cond then
+                        (r0 >= -(v $gamma2) /\ r0 < 0)
                     else
-                        (r0 == r_g /\ r1 == (r_q - r_g) / (v $gamma2 * 2) /\
-                        (r0 > -(v $gamma2) /\ r0 <= v $gamma2))) /\
+                        (r0 > -(v $gamma2) /\ r0 <= v $gamma2)) /\
                     (r1 >= 0 /\ r1 < (v $FIELD_MODULUS - 1) / (v $gamma2 * 2)))"#
             )
         });
@@ -749,14 +681,7 @@ pub fn decompose(
 #[hax_lib::ensures(|_| fstar!(r#"forall i. i < 8 ==>
     (let h = Seq.index ${hint}.f_values i in
     let result = Seq.index ${hint}_future.f_values i in
-    let r0, r1 = decompose_element $gamma2 (Seq.index ${simd_unit}.f_values i) in
-    if v h = 0 then
-        result = r1
-    else
-        (if v r0 > 0 then
-            v result = (v r1 + 1) % (4190208 / v $gamma2)
-        else
-            v result = (v r1 - 1) % (4190208 / v $gamma2)))"#))]
+    v result = Spec.MLDSA.Math.use_one_hint (v $gamma2) (v (Seq.index ${simd_unit}.f_values i)) (v h))"#))]
 pub fn use_hint(gamma2: Gamma2, simd_unit: &Coefficients, hint: &mut Coefficients) {
     let _hint0 = hint.clone();
     for i in 0..hint.values.len() {
@@ -764,14 +689,7 @@ pub fn use_hint(gamma2: Gamma2, simd_unit: &Coefficients, hint: &mut Coefficient
             fstar!(r#"
                 (forall j. j < v i ==> (let h = Seq.index ${_hint0}.f_values j in
                     let result = Seq.index ${hint}.f_values j in
-                    let r0, r1 = decompose_element $gamma2 (Seq.index ${simd_unit}.f_values j) in
-                    if v h = 0 then
-                        result = r1
-                    else
-                        (if v r0 > 0 then
-                            v result = (v r1 + 1) % (4190208 / v $gamma2)
-                        else
-                            v result = (v r1 - 1) % (4190208 / v $gamma2)))) /\
+                    v result = Spec.MLDSA.Math.use_one_hint (v $gamma2) (v (Seq.index ${simd_unit}.f_values j)) (v h))) /\
                 (forall j. j >= v i ==> (Seq.index ${hint}.f_values j == Seq.index ${_hint0}.f_values j /\
                     (v (Seq.index ${hint}.f_values j) == 0 \/ v (Seq.index ${hint}.f_values j) == 1)))"#
             )
