libcrux-ml-dsa/proofs/fstar/extraction/Libcrux_ml_dsa.Simd.Portable.Arithmetic.fst
@@ -382,18 +382,6 @@ let montgomery_multiply (lhs rhs: Libcrux_ml_dsa.Simd.Portable.Vector_type.t_Coe
 #push-options "--ext context_pruning --z3refresh --split_queries always"
 
 let power2round_element (t: i32) =
-  let _:Prims.unit =
-    if true
-    then
-      let _:Prims.unit =
-        Hax_lib.v_assert ((t >.
-              (Core.Ops.Arith.f_neg Libcrux_ml_dsa.Simd.Traits.v_FIELD_MODULUS <: i32)
-              <:
-              bool) &&
-            (t <. Libcrux_ml_dsa.Simd.Traits.v_FIELD_MODULUS <: bool))
-      in
-      ()
-  in
   let _:Prims.unit = logand_lemma Libcrux_ml_dsa.Simd.Traits.v_FIELD_MODULUS (t >>! mk_i32 31) in
   let e_t:i32 = t in
   let t:i32 =
@@ -411,26 +399,26 @@ let power2round_element (t: i32) =
   in
   let _:Prims.unit =
     assert (v t1 == (v t - 1 + pow2 12) / pow2 13);
-    assert ((v t - (Spec.Utils.mod_q (v t) (pow2 13))) / pow2 13 ==
-        (v t / pow2 13 - (Spec.Utils.mod_q (v t) (pow2 13)) / pow2 13));
+    assert ((v t - (Spec.Utils.mod_p (v t) (pow2 13))) / pow2 13 ==
+        (v t / pow2 13 - (Spec.Utils.mod_p (v t) (pow2 13)) / pow2 13));
     if v t % pow2 13 > pow2 12
     then
-      (assert (Spec.Utils.mod_q (v t) (pow2 13) == v t % pow2 13 - pow2 13);
-        assert ((Spec.Utils.mod_q (v t) (pow2 13)) / pow2 13 == (v t % pow2 13 - pow2 13) / pow2 13);
+      (assert (Spec.Utils.mod_p (v t) (pow2 13) == v t % pow2 13 - pow2 13);
+        assert ((Spec.Utils.mod_p (v t) (pow2 13)) / pow2 13 == (v t % pow2 13 - pow2 13) / pow2 13);
         assert ((v t % pow2 13 - pow2 13) / pow2 13 == (v t % pow2 13) / pow2 13 - pow2 13 / pow2 13
           );
         assert ((v t % pow2 13) / pow2 13 - pow2 13 / pow2 13 == - 1);
-        assert ((v t - (Spec.Utils.mod_q (v t) (pow2 13))) / pow2 13 == v t / pow2 13 + 1))
+        assert ((v t - (Spec.Utils.mod_p (v t) (pow2 13))) / pow2 13 == v t / pow2 13 + 1))
     else
-      (assert ((v t - (Spec.Utils.mod_q (v t) (pow2 13))) / pow2 13 == v t / pow2 13);
+      (assert ((v t - (Spec.Utils.mod_p (v t) (pow2 13))) / pow2 13 == v t / pow2 13);
         assert ((v t - 1 + pow2 12) / pow2 13 == v t / pow2 13));
-    assert (v t1 == (v t - (Spec.Utils.mod_q (v t) (pow2 13))) / pow2 13)
+    assert (v t1 == (v t - (Spec.Utils.mod_p (v t) (pow2 13))) / pow2 13)
   in
   let t0:i32 = t -! (t1 <<! Libcrux_ml_dsa.Constants.v_BITS_IN_LOWER_PART_OF_T <: i32) in
   let _:Prims.unit =
-    assert (v t0 == v t - ((v t - (Spec.Utils.mod_q (v t) (pow2 13))) / pow2 13) * pow2 13);
-    assert (v t0 == v t - (v t - (Spec.Utils.mod_q (v t) (pow2 13))));
-    assert (v t0 == Spec.Utils.mod_q (v t) (pow2 13))
+    assert (v t0 == v t - ((v t - (Spec.Utils.mod_p (v t) (pow2 13))) / pow2 13) * pow2 13);
+    assert (v t0 == v t - (v t - (Spec.Utils.mod_p (v t) (pow2 13))));
+    assert (v t0 == Spec.Utils.mod_p (v t) (pow2 13))
   in
   t0, t1 <: (i32 & i32)
 
@@ -458,16 +446,12 @@ let power2round (t0 t1: Libcrux_ml_dsa.Simd.Portable.Vector_type.t_Coefficients)
           let i:usize = i in
           (forall j.
               j < v i ==>
-              (let t0_1 =
-                  v (Seq.index e_t0.f_values j) % v Libcrux_ml_dsa.Simd.Traits.v_FIELD_MODULUS
-                in
-                let t0_2 = v (Seq.index t0.f_values j) in
-                t0_2 ==
-                Spec.Utils.mod_q t0_1 (pow2 (v Libcrux_ml_dsa.Constants.v_BITS_IN_LOWER_PART_OF_T)) /\
-                v (Seq.index t1.f_values j) ==
-                (t0_1 - t0_2) / pow2 (v Libcrux_ml_dsa.Constants.v_BITS_IN_LOWER_PART_OF_T) /\
-                t0_2 > - (pow2 (v Libcrux_ml_dsa.Constants.v_BITS_IN_LOWER_PART_OF_T - 1)) /\
-                t0_2 <= pow2 (v Libcrux_ml_dsa.Constants.v_BITS_IN_LOWER_PART_OF_T - 1))) /\
+              (let t0_v = v (Seq.index t0.f_values j) in
+                let t0_s, t1_s = Spec.MLDSA.Math.power2round (v (Seq.index e_t0.f_values j)) in
+                t0_v == t0_s /\ v (Seq.index t1.f_values j) == t1_s /\
+                Spec.Utils.is_intb_bt (pow2 (v Libcrux_ml_dsa.Constants.v_BITS_IN_LOWER_PART_OF_T -
+                        1))
+                  t0_v)) /\
           (forall j.
               j >= v i ==>
               (Seq.index t0.f_values j == Seq.index e_t0.f_values j /\
@@ -544,18 +528,6 @@ let infinity_norm_exceeds
           let result:bool = result in
           let i:usize = i in
           let coefficient:i32 = simd_unit.Libcrux_ml_dsa.Simd.Portable.Vector_type.f_values.[ i ] in
-          let _:Prims.unit =
-            if true
-            then
-              let _:Prims.unit =
-                Hax_lib.v_assert ((coefficient >.
-                      (Core.Ops.Arith.f_neg Libcrux_ml_dsa.Simd.Traits.v_FIELD_MODULUS <: i32)
-                      <:
-                      bool) &&
-                    (coefficient <. Libcrux_ml_dsa.Simd.Traits.v_FIELD_MODULUS <: bool))
-              in
-              ()
-          in
           let sign:i32 = coefficient >>! mk_i32 31 in
           let _:Prims.unit = logand_lemma (mk_i32 2 *! coefficient) sign in
           let normalized:i32 = coefficient -! (sign &. (mk_i32 2 *! coefficient <: i32) <: i32) in
@@ -645,35 +617,15 @@ let compute_one_hint (low high gamma2: i32) =
   then mk_i32 1
   else mk_i32 0
 
-val hint_counter_loop:
-  hint_1:t_Array i32 (mk_usize 8)
-  -> hint_2:t_Array i32 (mk_usize 8)
-  -> n:nat{n < 8} ->
-  Lemma
-   (requires
-      forall (i:nat). i < n ==> hint_1.[mk_usize i] == hint_2.[mk_usize i])
-    (ensures
-      Lib.LoopCombinators.repeati n (hint_counter hint_1) 0 ==
-        Lib.LoopCombinators.repeati n (hint_counter hint_2) 0)
-
-let rec hint_counter_loop hint_1 hint_2 n =
-  if n = 0 then begin
-    Lib.LoopCombinators.eq_repeati0 n (hint_counter hint_1) 0;
-    Lib.LoopCombinators.eq_repeati0 n (hint_counter hint_2) 0;
-    () end
-  else begin
-    hint_counter_loop hint_1 hint_2 (n - 1);
-    Lib.LoopCombinators.unfold_repeati n (hint_counter hint_1) 0 (n - 1);
-    Lib.LoopCombinators.unfold_repeati n (hint_counter hint_2) 0 (n - 1);
-    () end
-
 let compute_hint
       (low high: Libcrux_ml_dsa.Simd.Portable.Vector_type.t_Coefficients)
       (gamma2: i32)
       (hint: Libcrux_ml_dsa.Simd.Portable.Vector_type.t_Coefficients)
      =
   let one_hints_count:usize = mk_usize 0 in
-  let _:Prims.unit = Lib.LoopCombinators.eq_repeati0 0 (hint_counter hint.f_values) 0 in
+  let _:Prims.unit =
+    Lib.LoopCombinators.eq_repeati0 0 (Spec.MLDSA.Math.hint_counter hint.f_values) 0
+  in
   let hint, one_hints_count:(Libcrux_ml_dsa.Simd.Portable.Vector_type.t_Coefficients & usize) =
     Rust_primitives.Hax.Folds.fold_range (mk_usize 0)
       (Core.Slice.impl__len #i32
@@ -689,13 +641,12 @@ let compute_hint
           v i >= 0 /\ v i <= 8 /\
           (forall j.
               j < v i ==>
-              (let r = v (Seq.index hint.f_values j) in
-                let l = v (Seq.index low.f_values j) in
-                let h = v (Seq.index high.f_values j) in
-                if l > v gamma2 || l < - (v gamma2) || (l = - (v gamma2) && h <> 0)
-                then r = 1
-                else r = 0)) /\ v one_hints_count <= v i /\
-          v one_hints_count == Lib.LoopCombinators.repeati (v i) (hint_counter hint.f_values) 0)
+              (v (Seq.index hint.f_values j) =
+                Spec.MLDSA.Math.compute_one_hint (v (Seq.index low.f_values j))
+                  (v (Seq.index high.f_values j))
+                  (v gamma2))) /\ v one_hints_count <= v i /\
+          v one_hints_count ==
+          Lib.LoopCombinators.repeati (v i) (Spec.MLDSA.Math.hint_counter hint.f_values) 0)
       (hint, one_hints_count <: (Libcrux_ml_dsa.Simd.Portable.Vector_type.t_Coefficients & usize))
       (fun temp_0_ i ->
           let hint, one_hints_count:(Libcrux_ml_dsa.Simd.Portable.Vector_type.t_Coefficients & usize
@@ -726,8 +677,11 @@ let compute_hint
             Libcrux_ml_dsa.Simd.Portable.Vector_type.t_Coefficients
           in
           let _:Prims.unit =
-            hint_counter_loop hint.f_values e_hint_values (v i);
-            Lib.LoopCombinators.unfold_repeati (v i + 1) (hint_counter hint.f_values) 0 (v i)
+            Spec.MLDSA.Math.hint_counter_loop hint.f_values e_hint_values (v i);
+            Lib.LoopCombinators.unfold_repeati (v i + 1)
+              (Spec.MLDSA.Math.hint_counter hint.f_values)
+              0
+              (v i)
           in
           let one_hints_count:usize =
             one_hints_count +!
@@ -739,21 +693,9 @@ let compute_hint
   let hax_temp_output:usize = one_hints_count in
   hint, hax_temp_output <: (Libcrux_ml_dsa.Simd.Portable.Vector_type.t_Coefficients & usize)
 
-#push-options "--fuel 3 --z3rlimit 500 --ext context_pruning --z3refresh --split_queries always"
+#push-options "--fuel 3 --z3rlimit 1500 --ext context_pruning --z3refresh --split_queries always"
 
 let decompose_element (gamma2 r: i32) =
-  let _:Prims.unit =
-    if true
-    then
-      let _:Prims.unit =
-        Hax_lib.v_assert ((r >.
-              (Core.Ops.Arith.f_neg Libcrux_ml_dsa.Simd.Traits.v_FIELD_MODULUS <: i32)
-              <:
-              bool) &&
-            (r <. Libcrux_ml_dsa.Simd.Traits.v_FIELD_MODULUS <: bool))
-      in
-      ()
-  in
   let e_r:i32 = r in
   let _:Prims.unit = logand_lemma Libcrux_ml_dsa.Simd.Traits.v_FIELD_MODULUS (r >>! mk_i32 31) in
   let r:i32 =
@@ -773,7 +715,7 @@ let decompose_element (gamma2 r: i32) =
         assert (v result == ((v ceil_of_r_by_128_ * 11275) + pow2 23) / pow2 24);
         assert (v result == ((((v r + 127) / 128) * 11275) + pow2 23) / pow2 24);
         assert (v result == (v r - 1 + 95232) / 190464);
-        assert (v result == (v r - (Spec.Utils.mod_q (v r) 190464)) / 190464);
+        assert (v result == (v r - (Spec.Utils.mod_p (v r) 190464)) / 190464);
         assert (v result >= 0 /\ v result <= 44)
       in
       let _:Prims.unit =
@@ -798,7 +740,7 @@ let decompose_element (gamma2 r: i32) =
         assert (v result == ((v ceil_of_r_by_128_ * 1025) + pow2 21) / pow2 22);
         assert (v result == ((((v r + 127) / 128) * 1025) + pow2 21) / pow2 22);
         assert (v result == (v r - 1 + 261888) / 523776);
-        assert (v result == (v r - (Spec.Utils.mod_q (v r) 523776)) / 523776);
+        assert (v result == (v r - (Spec.Utils.mod_p (v r) 523776)) / 523776);
         assert (v result >= 0 /\ v result <= 16)
       in
       let _:Prims.unit = logand_mask_lemma result 4 in
@@ -837,14 +779,14 @@ let decompose_element (gamma2 r: i32) =
   let _:Prims.unit =
     assert (v e_r0 > 4190208 ==> v r0 == v e_r0 - 8380417);
     assert (v e_r0 <= 4190208 ==> v r0 == v e_r0);
-    if v r - (Spec.Utils.mod_q (v r) (v alpha)) = 8380416
+    if v r - (Spec.Utils.mod_p (v r) (v alpha)) = 8380416
     then
       (assert (v r1 == 0);
-        assert (v r0 == (Spec.Utils.mod_q (v r) (v alpha)) - 1);
+        assert (v r0 == (Spec.Utils.mod_p (v r) (v alpha)) - 1);
         assert (v r0 >= - (v gamma2) /\ v r0 < 0))
     else
-      (assert (v r1 == (v r - (Spec.Utils.mod_q (v r) (v alpha))) / v alpha);
-        assert (v r0 == Spec.Utils.mod_q (v r) (v alpha));
+      (assert (v r1 == (v r - (Spec.Utils.mod_p (v r) (v alpha))) / v alpha);
+        assert (v r0 == Spec.Utils.mod_p (v r) (v alpha));
         assert (v r0 > - (v gamma2) /\ v r0 <= v gamma2));
     assert (v r1 >= 0 /\ v r1 < 8380416 / (v alpha))
   in
@@ -882,7 +824,6 @@ let decompose
       (gamma2: i32)
       (simd_unit low high: Libcrux_ml_dsa.Simd.Portable.Vector_type.t_Coefficients)
      =
-  let e_simd_unit0:Libcrux_ml_dsa.Simd.Portable.Vector_type.t_Coefficients = simd_unit in
   let high, low:(Libcrux_ml_dsa.Simd.Portable.Vector_type.t_Coefficients &
     Libcrux_ml_dsa.Simd.Portable.Vector_type.t_Coefficients) =
     Rust_primitives.Hax.Folds.fold_range (mk_usize 0)
@@ -901,13 +842,11 @@ let decompose
             (let r = v (Seq.index simd_unit.f_values j) in
               let r0 = v (Seq.index low.f_values j) in
               let r1 = v (Seq.index high.f_values j) in
-              let r_q = r % v Libcrux_ml_dsa.Simd.Traits.v_FIELD_MODULUS in
-              let r_g = Spec.Utils.mod_q r_q (v gamma2 * 2) in
-              (if r_q - r_g = v Libcrux_ml_dsa.Simd.Traits.v_FIELD_MODULUS - 1
-                then (r0 == r_g - 1 /\ r1 == 0 /\ (r0 >= - (v gamma2) /\ r0 < 0))
-                else
-                  (r0 == r_g /\ r1 == (r_q - r_g) / (v gamma2 * 2) /\
-                    (r0 > - (v gamma2) /\ r0 <= v gamma2))) /\
+              let r0_s, r1_s, cond = Spec.MLDSA.Math.decompose (v gamma2) r in
+              r0 = r0_s /\ r1 = r1_s /\
+              (if cond
+                then (r0 >= - (v gamma2) /\ r0 < 0)
+                else (r0 > - (v gamma2) /\ r0 <= v gamma2)) /\
               (r1 >= 0 /\ r1 < (v Libcrux_ml_dsa.Simd.Traits.v_FIELD_MODULUS - 1) / (v gamma2 * 2)))
       )
       (high, low
@@ -983,13 +922,8 @@ let uuse_hint
               j < v i ==>
               (let h = Seq.index e_hint0.f_values j in
                 let result = Seq.index hint.f_values j in
-                let r0, r1 = decompose_element gamma2 (Seq.index simd_unit.f_values j) in
-                if v h = 0
-                then result = r1
-                else
-                  (if v r0 > 0
-                    then v result = (v r1 + 1) % (4190208 / v gamma2)
-                    else v result = (v r1 - 1) % (4190208 / v gamma2)))) /\
+                v result =
+                Spec.MLDSA.Math.use_one_hint (v gamma2) (v (Seq.index simd_unit.f_values j)) (v h))) /\
           (forall j.
               j >= v i ==>
               (Seq.index hint.f_values j == Seq.index e_hint0.f_values j /\
