libcrux-ml-kem/proofs/fstar/spec/Spec.Utils.fsti
@@ -247,5 +247,7 @@ let inv_ntt_spec #len (vec_in: t_Array i16 len) (zeta: int) (i: nat{i < v len}) 
    (((v (Seq.index vec_in j) - v (Seq.index vec_in i)) * zeta * 169) % 3329))
 
 (* Wrap-around modulo: wraps into ]-p/2; p/2] *)
-let mod_q (v:int) (p:int{p>0/\ p%2=0}) : Tot int =
+let mod_p (v:int) (p:int{p>0/\ p%2=0}) : Tot int =
   let m = v % p in if m > p/2 then m - p else m
+
+let is_intb_bt (l:nat) (x:int) = (x > -l) && (x <= l)
